# Formula Sheet

$$
\begin{align}
&&\mathbb{K}\mathbf{v} &= \omega^{2}\mathbb{M}\mathbf{v} &&  \\[1em]
\Lambda\mathbf{v} &= \lambda\mathbf{v} & \det(\Lambda-\lambda\text{Id})\mathbf{v} &= 0 & \Lambda &=\mathbb{M}^{-1}\mathbb{K}\qc\lambda = \omega^{2}
\end{align}
$$

$$
\begin{align}
\mathbf{v} & = \sum\limits_{\omega_{\alpha}\neq 0}\mathbf{v}^{\alpha}\left(V_{\alpha}\cos (\omega_{\alpha}t)+ D_{\alpha}\sin (\omega_{\alpha}t) \right) + \sum\limits_{\omega_{\alpha}= 0}\mathbf{v}^{\alpha}(C_{\alpha}+ D_{\alpha}t)
\end{align}
$$

The second sum only applies if and only if there are some $\omega_{\alpha}= 0$.

$$
\begin{align}
\dot{\mathbf{p}} & = \pdv{L}{\mathbf{q}}\qc \mathbf{p} = \pdv{L}{\dot{\mathbf{q}}}.
\end{align}
$$

We solve for $\mathbf{p}= \mathbf{p}(\dot{\mathbf{q}}, \mathbf{q}, t)$ for $\dot{\mathbf{q}}$ and express $\dot{\mathbf{q}} = \dot{\mathbf{q}}(\mathbf{p}, \mathbf{q}\mathbf{t})$.

$$
\begin{align}
H (\mathbf{q}, \mathbf{p}\mathbf{t}) & = \mathbf{p}\cdot \dot{\mathbf{q}} - L \\[1 em]
\dot{\mathbf{p}} & = -\pdv{H}{\mathbf{q}}\qc \dot{\mathbf{q}} = \pdv{H}{\mathbf{p}}.
\end{align}
$$

$$
\begin{align}
\{F, G\} & = \pdv{F}{\mathbf{q}}\cdot \pdv{G}{\mathbf{p}}- \pdv{F}{\mathbf{p}}\cdot \pdv{G}{\mathbf{q}} \\[1 em]
\dot{p}_{\alpha} & = \{p_{\alpha}, H \}\qc \dot{q}_{\alpha} = \{q^{\alpha}, H\}
\end{align}
$$

$$
\begin{align}
\comm{X}{Y} & = XY-YX,
\end{align}
$$

apply to an arbitrary function $f$ and find the correlation.

$$
\begin{align}
\theta & = \theta_{\alpha}(\mathbf{\xi})\dd{\xi}^{\alpha} \\[1 em]
\theta (X) & = \theta_{\alpha}(\mathbf{\xi})X^{\alpha}(\mathbf{\xi})
\end{align}
$$

$$
\begin{align}
\omega (X, Y) & = -\omega (Y, X) \\
\omega (aX_{1} + bX_{2}, Y) & = a\omega (X_{1}, Y) + b \omega (X_{2}, Y).
\end{align}
$$

$$
\begin{align}
i_{X}\theta & = \theta (X) = \theta_{\alpha}X^{\alpha} \\[1 em]
i_{X}\omega (Y) & = \omega (X, Y) \\[1 em]
i_{X}(\theta \wedge \psi) & = \theta (X)\psi-\psi (X)\theta \\[1 em]
(\theta \wedge \psi)(X, Y) & = i_{Y}i_{X}(\theta \wedge \psi) = \theta (X)\psi (Y)-\psi (X)\theta (Y).
\end{align}
$$

$$
\begin{align}
\dd{f (X)} & = \pdv{f}{\xi^{\alpha}}\dd{\xi^{\alpha}}\\[1 em]
\dd{\theta} & = \pdv{\theta_{\alpha}}{\xi^{\beta}}\dd{x^{\beta}}\wedge \dd{x^{\alpha}}
\end{align}
$$

Closed implies $\dd \theta = 0$, exact implies $\theta = \dd{\zeta}$. $\dd{\dd{\theta}}= 0$.

Generating functions:

$$
\begin{align}
\pdv{F}{q^{\alpha}}& = p_{\alpha} - P_{\beta}\pdv{Q^{\beta}}{q^{\alpha}} \\
\pdv{F}{p_{\alpha}} & = -P_{\beta}\pdv{Q^{\beta}}{p_{\alpha}} \\[1 em]
K & = H + \pdv{F_{0}}{t}+ P_{\beta}\pdv{Q^{\beta}}{t}.
\end{align}
$$

Type 1: $(q, Q)$

$$
\begin{align}
p_{\alpha} & = \pdv{F_{1}}{q^{\alpha}} \\
P_{\alpha} & = -\pdv{F_{1}}{Q^{\alpha}} \\[1 em]
K & = H + \pdv{F_{1}}{t}
\end{align}
$$

Type 2: $(q, P)$

$$
\begin{align}
F & = F_{2} - P \cdot Q (q, P, t) \\[1 em]
p_{\alpha} & = \pdv{F_{2}}{q^{\alpha}} \\
Q_{\alpha} & = \pdv{F_{2}}{P_{\alpha}} \\[1 em]
K & = H + \pdv{F_{2}}{t}
\end{align}
$$

Type 3: $(p, Q)$

$$
\begin{align}
F_{3} & = F_{3}-q (p, Q)\cdot p \\[1 em]
q^{\alpha} & = -\pdv{F_{3}}{p_{\alpha}} \\
P_{\alpha} & = -\pdv{F_{3}}{Q^{\alpha}} \\[1 em]
K & = H + \pdv{F_{3}}{t}
\end{align}
$$

Type 4: $(p, P)$

$$
\begin{align}
F & = F_{4}+ q (p, P)\cdot p-Q (p, P)\cdot P \\[1 em]
q^{\alpha} & = -\pdv{F_{4}}{p_{\alpha}} \\
Q^{\alpha} & = \pdv{F_{4}}{P_{\alpha}} \\[1 em]
K & = H + \pdv{F_{4}}{t}
\end{align}
$$