We begin this chapter by reviewing some of the concepts of Newtonian and special-relativistic viewpoints of space and time. To specify any one event uniquely, we assign to it three spatial coordinates and one time coordinate, which themselves are defined with respect to some reference frame $S$. All together, the four coordinates $(t, x, y, z)$ then label events in space and time (again with respect to the reference frame $S$.)

# Inertial Frames and the Principle of Relativity

Clearly, we are free to label any events not only with respect to $S$, but any other frame $S'$. $S'$ may be oriented and/or moving with respect to $S$ in some arbitrary manner. There exist, however, a class of reference frames that are in a sense, preferred. These are called *inertial frames*, and they are defined as frames in which Newton's first law holds, i.e. a free particle is either at rest or moving with constant velocity with respect to our frame. Mathematically, we want our Cartesian coordinates to be such that

$$
\dv[2]{x}{t}= \dv[2]{y}{t}= \dv[2]{z}{t}= 0.
$$

Therefore, in the absence of gravity, if $S$ and $S'$ are two inertial reference frames, then $S'$ can only differ from $S$ by
1. A translation,
2. a  rotation, or
3. a motion of one frame with respect to the other at a *constant* velocity.

This concept is fundamental to the *principle of relativity*, which states that the laws of physics take the same form in every inertial frame.

The difference between Newton's description and that of special relativity is how the coordinates of an event $P$ in two inertial frames are related. Let us consider two frames, $S$ and $S'$, where $S'$ is moving along the $x$-axis of $S$ at constant speed $v$ and the axes of $S$ and $S'$ coincide at time $t = t' = 0$. The primed coordinates of an event $P$ with respect to $S'$ are related to the unprimed coordinates in $S$ via a linear transformation of the form

$$
\begin{align}
t' & = At + Bx \\[1 em]
x' & = Dt + Ex \\[1 em]
y' & = y \\[1 em]
z' & = z.
\end{align}
$$

Since we require that $x' = 0$ corresponds to $x = vt$ and that $x = 0$ corresponds to $x' =-vt$, we find that $D =-Ev$ and $D =-Av$, and so $A = E$ and we have

$$
\begin{align}
t' & = At + Bx \\[1 em]
x' & = A (x-vt) \\[1 em]
y' & = y \\[1 em]
z' & = z
\end{align}
$$